Makefile
@@ -203,7 +203,7 @@ CONCUR=MultiLibs.v CMulti.v AsmMulti.v \
        InjpAccoComp.v VCompBig.v \
        SimplLocalsproofC.v CminorgenproofC.v InliningproofC.v \
        InvariantC.v StackingproofC.v \
-       ConstpropproofC.v CSEproofC.v \
+       ConstpropproofC.v CSEproofC.v DeadcodeproofC.v\
        Composition.v
 
 
